Weakened inv_unseen a little and used it to clear some admits. Pushed through.

sample_mark/dijk_pq_arr_spec.v
@@ -55,6 +55,8 @@ Definition inv_popped (g: LGraph) src prev priq dist dst :=
       path_in_popped g priq dist path /\
       path_globally_optimal g src dst path).
 
+
+(*
 Definition inv_popped_weak (g: LGraph) src prev priq dist dst u :=
   In dst (get_popped priq) ->
   (Znth dst dist = inf /\
@@ -80,6 +82,7 @@ Definition inv_popped_weak (g: LGraph) src prev priq dist dst u :=
       path_correct g prev dist src dst path /\
       path_in_popped g priq dist path /\ (* why don't I need weak? *)
       path_globally_optimal g src dst path).
+*)
 
 Definition inv_unpopped g src prev priq dist dst :=
   Znth dst priq < inf ->
@@ -110,19 +113,19 @@ Definition inv_unpopped_weak g src prev priq dist dst u :=
      Znth dst dist <=
      careful_add (Znth mom' dist) (Znth dst (Znth mom' (graph_to_mat g)))).
   
-Definition inv_unseen g prev priq dist dst :=
+Definition inv_unseen g priq dist dst :=
   Znth dst priq = inf ->
   Znth dst dist = inf /\
-  Znth dst prev = inf /\
+  (* Znth dst prev = inf /\ *)
   forall m, In m (get_popped priq) ->
             careful_add 
               (Znth m dist)
               (Znth dst (Znth m (graph_to_mat g))) = inf.
 
-Definition inv_unseen_weak g prev priq dist dst u :=
+Definition inv_unseen_weak g priq dist dst u :=
   Znth dst priq = inf ->
   Znth dst dist = inf /\
-  Znth dst prev = inf /\
+  (* Znth dst prev = inf /\ *)
   forall m, In m (get_popped priq) ->
             m <> u ->
             careful_add
@@ -134,7 +137,7 @@ Definition dijkstra_correct (g: LGraph) (src : VType) (prev priq dist: list VTyp
     vvalid g dst ->
     inv_popped g src prev priq dist dst /\
     inv_unpopped g src prev priq dist dst /\
-    inv_unseen g prev priq dist dst.
+    inv_unseen g priq dist dst.
 
 Definition push_spec :=
   DECLARE _push
